+ result

Opcodes.fst
@@ -15,33 +15,35 @@ assume val hash_ripemd160: #a:eqtype -> input : a -> Tot(output: a)
 
 (* 118 *)
 val op_dup : #a: eqtype -> st_before: stackBC a{Stack.length st_before > 0 /\ Stack.capacity st_before > 0}  -> 
-				line_before: seq nat{Seq.length line_before > 0 /\ (Seq.head line_before = 118)}
+				line_before: seq nat{Seq.length line_before > 0 /\ (Seq.head line_before = 118)} 
+				-> result_before : bool
 				-> Tot (st: stackBC a 
 								{Stack.length st > 1 /\ 
 								(Stack.index st 0) = (Stack.index st 1) /\ 
 								Stack.length st = Stack.length st_before + 1}	* 
-						line : seq nat {Seq.length line = Seq.length line_before - 1 }) 
+						line : seq nat {Seq.length line = Seq.length line_before - 1 } * result: bool) 
 
-let op_dup #a st_before line_before = 
+let op_dup #a st_before line_before result_before = 
 	let pop = Stack.pop st_before in 
 	let element = fst pop in 
 	let stack_after_pop = snd pop in 
 	let stack_push1 = Stack.push stack_after_pop element in 
 	let stack_push2 = Stack.push stack_push1 element in 
-	let line = Seq.tail line_before in (stack_push2, line)
+	let line = Seq.tail line_before in (stack_push2, line, result_before)
 
 val op_hash160 : #a: eqtype -> st_before : stackBC a{Stack.length st_before > 0} -> 
 				line_before : seq nat {Seq.length line_before > 0 /\ (Seq.head line_before = 169)}
+				-> result_before : bool 
 				-> Tot(st: stackBC a 
 						{Stack.length st > 0  /\
 						Stack.index st 0 = (hash_ripemd160(hash_sha256 (Stack.index st_before 0))) /\
 						Stack.length st = Stack.length st_before} * 
-					line : seq nat {Seq.length line = Seq.length line_before - 1})
+					line : seq nat {Seq.length line = Seq.length line_before - 1} * result: bool)
 
-let op_hash160 #a st_before line_before = 
-	let pop = Stack.pop st_before in 
-	let element = fst pop in 
-	let stack_after_pop = snd pop in 
-	let element = hash_ripemd160(hash_sha256 element) in 
-	let stack_push1 = Stack.push stack_after_pop element in 
-	let line = Seq.tail line_before in (stack_push1, line)
+let op_hash160 #a st_before line_before result_before = 
+		let pop = Stack.pop st_before in 
+		let element = fst pop in 
+		let stack_after_pop = snd pop in 
+		let element = hash_ripemd160(hash_sha256 element) in 
+		let stack_push1 = Stack.push stack_after_pop element in 
+		let line = Seq.tail line_before in (stack_push1, line, result_before)
